Add eager transitions to x86 TSO operational model (#88)
Co-authored-by: Thibaut Pérami <thibaut.perami@cl.cam.ac.uk>

ArchSemX86/tests/X86OperationalModelTest.v
@@ -136,9 +136,18 @@ Module EOR.
       archState.address_space := () |}.
 
   Definition test_results :=
-    x86_operational_modelc 2 x86_sem 1%nat termCond initState.
+    x86_operational_modelc 2 x86_sem false 1%nat termCond initState.
 
   Goal reg_extract RAX 0%fin <$> test_results = Listset [Ok 0x110%Z].
+  Proof.
+    vm_compute (_ <$> _).
+    reflexivity.
+  Qed.
+
+  Definition test_results_eager :=
+    x86_operational_modelc 2 x86_sem true 1%nat termCond initState.
+
+  Goal reg_extract RAX 0%fin <$> test_results_eager = Listset [Ok 0x110%Z].
     Proof.
     vm_compute (_ <$> _).
     reflexivity.
@@ -195,7 +204,17 @@ Module MP.
   Definition fuel := 12%nat.
 
   Definition test_results :=
-    x86_operational_modelc fuel x86_sem n_threads termCond initState.
+    x86_operational_modelc fuel x86_sem false n_threads termCond initState.
+
+  Goal elements (regs_extract [(1%fin, RAX); (1%fin, RBX)] <$> test_results) ≡ₚ
+    [Ok [0x0%Z;0x0%Z]; Ok [0x0%Z;0x1%Z]; Ok [0x1%Z; 0x1%Z]].
+  Proof.
+    vm_compute (elements _).
+    apply NoDup_Permutation; try solve_NoDup; set_solver.
+  Qed.
+
+  Definition test_results_eager :=
+    x86_operational_modelc fuel x86_sem true n_threads termCond initState.
 
   Goal elements (regs_extract [(1%fin, RAX); (1%fin, RBX)] <$> test_results) ≡ₚ
     [Ok [0x0%Z;0x0%Z]; Ok [0x0%Z;0x1%Z]; Ok [0x1%Z; 0x1%Z]].
@@ -256,9 +275,19 @@ Module SB.
   Definition fuel := 12%nat.
 
   Definition test_results :=
-    x86_operational_modelc fuel x86_sem n_threads termCond initState.
+    x86_operational_modelc fuel x86_sem false n_threads termCond initState.
 
   Goal elements (regs_extract [(0%fin, RAX); (1%fin, RAX)] <$> test_results) ≡ₚ
+    [Ok [0x0%Z;0x0%Z]; Ok [0x0%Z;0x1%Z]; Ok [0x1%Z; 0x0%Z]; Ok [0x1%Z; 0x1%Z]].
+  Proof.
+    vm_compute (elements _).
+    apply NoDup_Permutation; try solve_NoDup; set_solver.
+  Qed.
+
+  Definition test_results_eager :=
+    x86_operational_modelc fuel x86_sem true n_threads termCond initState.
+
+  Goal elements (regs_extract [(0%fin, RAX); (1%fin, RAX)] <$> test_results_eager) ≡ₚ
     [Ok [0x0%Z;0x0%Z]; Ok [0x0%Z;0x1%Z]; Ok [0x1%Z; 0x0%Z]; Ok [0x1%Z; 0x1%Z]].
   Proof.
     vm_compute (elements _).
@@ -316,13 +345,23 @@ Module R_PO_MFENCE.
 
   Definition fuel := 12%nat.
 
+  Definition result_extraction (test_result : archModel.res ∅ n_threads termCond) :=
+    [reg_extract RAX 1%fin test_result; mem_extract 0x1200 8 test_result].
+
   Definition test_results :=
-    x86_operational_modelc fuel x86_sem n_threads termCond initState.
+    x86_operational_modelc fuel x86_sem false n_threads termCond initState.
 
-  Definition result_extractions :=
-    (λ test_result, [(reg_extract RAX 1%fin test_result); (mem_extract 0x1200 8 test_result)]) <$> test_results.
+  Goal elements (result_extraction <$> test_results) ≡ₚ
+    [[Ok 0x0%Z; Ok 0x1%Z]; [Ok 0x1%Z; Ok 0x1%Z]; [Ok 0x1%Z; Ok 0x2%Z]].
+  Proof.
+    vm_compute (elements _).
+    apply NoDup_Permutation; try solve_NoDup; set_solver.
+  Qed.
 
-  Goal elements result_extractions ≡ₚ
+  Definition test_results_eager :=
+    x86_operational_modelc fuel x86_sem true n_threads termCond initState.
+
+  Goal elements (result_extraction <$> test_results) ≡ₚ
     [[Ok 0x0%Z; Ok 0x1%Z]; [Ok 0x1%Z; Ok 0x1%Z]; [Ok 0x1%Z; Ok 0x2%Z]].
   Proof.
     vm_compute (elements _).
@@ -397,8 +436,10 @@ Module IRIW.
 
   Definition fuel := 12%nat.
 
+  (* Non-eager runner is too slow (> 10s), we're not running it here *)
+
   Definition test_results :=
-    x86_operational_modelc fuel x86_sem n_threads termCond initState.
+    x86_operational_modelc fuel x86_sem true n_threads termCond initState.
 
   Goal elements (regs_extract [(1%fin, RAX); (1%fin, RBX); (3%fin, RAX); (3%fin, RBX)] <$> test_results) ≡ₚ
     [Ok [0x0%Z; 0x0%Z; 0x0%Z; 0x0%Z]; Ok [0x0%Z; 0x0%Z; 0x0%Z; 0x1%Z]; Ok [0x0%Z; 0x0%Z; 0x1%Z; 0x0%Z]; Ok [0x0%Z; 0x0%Z; 0x1%Z; 0x1%Z];
