ArchSemX86/OperationalX86TSO.v
@@ -44,56 +44,53 @@ From stdpp Require Import base options.
 
 Require Import X86Inst.
 
-(** this is an implementation of the x86-TSO operational concurrency model,
+(** This is an implementation of the x86-TSO operational concurrency model,
     as defined in https://www.cl.cam.ac.uk/~pes20/weakmemory/x86tso-paper.pdf *)
 
-
-
-(** * TSO Model Types *)
-
-Record addr_val : Type := {
-    addr: address;
-    size: N; (* IN BYTES *)
-    val: bv (8 * size)
-  }.
-
-(* archState + extra fields (buffer and lock)*)
-Record machine_state {threads: nat} := {
-    regs : vec registerMap threads; (* Registers for each thread *)
-    mem : memoryMap;
-
-    (* Store buffer for each thread. Each buffer is a list of address-value
-       tuples, oldest first *)
-    buf : vec (list addr_val) threads;
-
-    (* Global machine lock, indicating when some thread has exclusive access to
-       memory *)
-    lock : option (fin threads);
-
-    (* Set of memory addresses that have been written to *)
-    memWritten : gset address;
-
-    (* Whether a thread is terminated, but not necessarily flushed *)
-    termThreads : vec bool threads;
-  }.
-Arguments machine_state : clear implicits.
-
-(** * TSO Model *)
 Section Model.
-  Context {threads: nat}.
+  (** The number of hardware threads *)
+  Context {threads : nat}.
 
-  Notation mstate_threads := (machine_state threads).
+  (** * Types *)
 
+  (** A memory entry in a write-buffer *)
+  Record addr_val := {
+      addr: address;
+      size: N; (* IN BYTES *)
+      val: bv (8 * size)
+    }.
+
+  (** The TSO model internal state *)
+  Record mstate := {
+      regs : vec registerMap threads; (* Registers for each thread *)
+      mem : memoryMap;
+
+      (* Store buffer for each thread. Each buffer is a list of address-value
+        tuples, oldest first *)
+      buf : vec (list addr_val) threads;
+
+      (* Global machine lock, indicating when some thread has exclusive access to
+        memory *)
+      lock : option (fin threads);
+
+      (* Set of memory addresses that have been written to *)
+      memWritten : gset address;
+
+      (* Whether a thread is terminated, but not necessarily flushed *)
+      termThreads : vec bool threads;
+    }.
+
+  (** * Helper functions *)
 
   (** ** Register functions *)
 
-  Definition read_reg (tid : fin threads) (reg : reg) (state : mstate_threads) :
+  Definition read_reg (tid : fin threads) (reg : reg) (state : mstate) :
       option (reg_type reg) :=
     let regMap := (regs state !!! tid) in
     dmap_lookup reg regMap.
 
   Definition write_reg (tid : fin threads) (reg : reg) (val : reg_type reg)
-      (state : mstate_threads) : mstate_threads :=
+      (state : mstate) : mstate :=
     set (lookup_total tid ∘ regs) (dmap_insert reg val) state.
 
 
@@ -101,19 +98,19 @@ Section Model.
   (** ** Buffer functions *)
 
   Definition no_pending (x : address) (tid : fin threads)
-      (state : mstate_threads) : bool :=
+      (state : mstate) : bool :=
     let buffer := buf state !!! tid in
     bool_decide (∀ av ∈ buffer, addr av ≠ x).
 
-  Definition buffer_empty (tid : fin threads) (m : mstate_threads) : bool :=
+  Definition buffer_empty (tid : fin threads) (m : mstate) : bool :=
     if buf m !!! tid is [] then true else false.
 
-  Definition all_buffers_empty (state: mstate_threads): bool :=
+  Definition all_buffers_empty (state : mstate) : bool :=
     bool_decide (∀ t : fin threads, buffer_empty t state).
 
   Fixpoint read_from_write_buffer_inner (rev_buffer : list addr_val)
       (goal_addr: address) (goal_size : N) :
-      Exec.t mstate_threads string (option (bv (8 * goal_size))) :=
+      Exec.t mstate string (option (bv (8 * goal_size))) :=
     (* Allow a direct match to be store-forwarded
        if it is the most recent write to all relevant addresses.
        Underapproximation of store buffering.
@@ -134,13 +131,13 @@ Section Model.
     end.
 
   Definition read_from_write_buffer (tid : fin threads) (addr : address) (size : N) :
-      Exec.t mstate_threads string (option (bv (8 * size))) :=
+      Exec.t mstate string (option (bv (8 * size))) :=
     buffer ← mget ((.!!! tid) ∘ buf);
     (* Reverse buffer so that we see most recent writes first *)
     read_from_write_buffer_inner (rev buffer) addr size.
 
   Fixpoint add_to_mem_written (addr : address) (size : nat) :
-      Exec.t mstate_threads string unit :=
+      Exec.t mstate string unit :=
     match size with
     | S size =>
         (* Add addr to the set of addresses that have been written to in memory*)
@@ -151,19 +148,19 @@ Section Model.
     end.
 
   Definition add_to_write_buffer (tid : fin threads) (addr : address)
-      (size : N) (val : bv (8 * size)) (state : mstate_threads) : mstate_threads :=
+      (size : N) (val : bv (8 * size)) (state : mstate) : mstate :=
     set ((.!!! tid) ∘ buf) (.++ [{| addr := addr; size := size; val := val |}])
       state.
 
 
   (** ** Memory functions *)
 
-  Definition mem_addr_modified (addr : address) (size : N) (state : mstate_threads) : bool :=
+  Definition mem_addr_modified (addr : address) (size : N) (state : mstate) : bool :=
     (* Returns true if address modified in memory or written to in a store buffer *)
     bool_decide (∃ a ∈ addr_range addr size, a ∈ memWritten state).
 
   Definition write_mem (addr : address) (size : N) (val : bv (8 * size)) :
-      Exec.t mstate_threads string unit :=
+      Exec.t mstate string unit :=
     (* Check if memory address is mapped*)
     opt ← mget (mem_lookup addr size ∘ mem);
     guard_or "Memory isn't mapped to write" (is_Some opt);;
@@ -174,7 +171,7 @@ Section Model.
   (** ** Buffer and Memory functions *)
 
   Definition read_mem_with_store_forwarding (tid : fin threads) (addr : address)
-      (size : N) : Exec.t mstate_threads string (bv (8 * size)) :=
+      (size : N) : Exec.t mstate string (bv (8 * size)) :=
     (* Attempt store forwarding *)
     opt ← read_from_write_buffer tid addr size;
     if opt is Some read then
@@ -186,7 +183,7 @@ Section Model.
       mret read.
 
   Fixpoint write_buffer_to_mem (buffer: list addr_val) (tid: fin threads) :
-      Exec.t mstate_threads string unit :=
+      Exec.t mstate string unit :=
     match buffer with
     | [] => mret ()
     | h :: t =>
@@ -194,7 +191,7 @@ Section Model.
         write_buffer_to_mem t tid
     end.
 
-  Definition empty_write_buffer (tid : fin threads) : Exec.t mstate_threads string unit :=
+  Definition empty_write_buffer (tid : fin threads) : Exec.t mstate string unit :=
     buffer ← mget ((.!!! tid) ∘ buf);
     (* Write all buffer contents to memory *)
     write_buffer_to_mem buffer tid;;
@@ -204,19 +201,19 @@ Section Model.
 
   (** ** Lock functions *)
 
-  Definition blocked (tid : fin threads) (m : mstate_threads) : bool :=
+  Definition blocked (tid : fin threads) (m : mstate) : bool :=
     if lock m is Some tid' then bool_decide (tid ≠ tid')
     else false.
 
-  Definition thread_has_lock (tid : fin threads) (m : mstate_threads) : bool :=
+  Definition thread_has_lock (tid : fin threads) (m : mstate) : bool :=
     if lock m is Some tid' then bool_decide (tid = tid')
     else false.
 
-  Definition acquire_lock (tid : fin threads) (state : mstate_threads) : mstate_threads :=
+  Definition acquire_lock (tid : fin threads) (state : mstate) : mstate :=
     setv lock (Some tid) state.
 
   Definition acquire_lock_conditional (tid : fin threads) :
-      Exec.t mstate_threads string unit :=
+      Exec.t mstate string unit :=
     (* Ensure thread can acquire lock: a thread (including thread tid) might already have the lock*)
     lock_status ← mget lock;
     guard_discard (lock_status = None);;
@@ -226,11 +223,11 @@ Section Model.
     (* Acquire lock *)
     mSet (acquire_lock tid).
 
-  Definition release_lock (tid : fin threads) (state : mstate_threads) : mstate_threads :=
+  Definition release_lock (tid : fin threads) (state : mstate) : mstate :=
     setv lock None state.
 
   Definition release_lock_conditional (tid : fin threads) :
-      Exec.t mstate_threads string unit :=
+      Exec.t mstate string unit :=
     (* Make sure we have the lock before releasing it *)
     state ← mGet;
     guard_discard (thread_has_lock tid state);;
@@ -240,13 +237,14 @@ Section Model.
     mSet (release_lock tid).
 
 
+  (** * Model transitions *)
 
   (** ** Run outcomes *)
 
   Section RunOutcome.
-    Context (tid : fin threads).
+    Context (tid : fin threads) (eager : bool).
 
-    Equations run_outcome (call : outcome) : Exec.t mstate_threads string (eff_ret call) :=
+    Equations run_outcome (call : outcome) : Exec.t mstate string (eff_ret call) :=
     | RegRead reg racc =>
         opt ← mget (read_reg tid reg);
         othrow ("Register " ++ pretty reg ++ " not found")%string opt
@@ -266,6 +264,8 @@ Section Model.
           read ← othrow ("Memory not found at " ++ pretty addr)%string opt;
           mret (Ok (read, 0%bv))
         else if is_explicit macc then
+          (* Cannot eagerly perform memory reads*)
+          guard_discard (negb eager);;
           (* Can't explicitly read from memory if we are blocked (some other
              thread has the lock) *)
           is_blocked ← mget (blocked tid);
@@ -285,10 +285,19 @@ Section Model.
         (* Add write to write buffer *)
         mSet (add_to_write_buffer tid addr size val);;
         (* Handle atomic case (release lock) *)
-        (if is_atomic_rmw macc then release_lock_conditional tid else mret ());;
+        (if is_atomic_rmw macc then
+          if eager then
+            (* Must discard outcome if eager, as release_lock_conditional requires
+              the store buffer to be emptied to complete *)
+            mdiscard
+          else release_lock_conditional tid
+        else mret ());;
         mret (Ok ())
     | MemWrite _ _ _ => mthrow "Unsupported MemWrite"
     | Barrier Barrier_MFENCE =>
+        (* Cannot eagerly perform memory barriers that do something*)
+        guard_discard (negb eager);;
+
         (* Write buffer (of thread tid) must be emptied before this instruction
            can complete. *)
         is_blocked ← mget (blocked tid);
@@ -301,7 +310,7 @@ Section Model.
 
   (** ** Flushing transition *)
   Definition flush_one_item_buffer (tid : fin threads) :
-      Exec.t mstate_threads string unit :=
+      Exec.t mstate string unit :=
     buffer ← mget ((.!!! tid) ∘ buf);
     match buffer with
     | [] => mdiscard
@@ -312,73 +321,181 @@ Section Model.
         msetv ((.!!! tid) ∘ buf) t
     end.
 
-  (** ** Top level transition *)
-  Definition step (isem : iMon ()) (term : terminationCondition threads):
-      Exec.t mstate_threads string () :=
+  Context (isem : iMon ()) (term : terminationCondition threads).
+
+  (** ** Execution step transition *)
+  Definition execution_step (tid : fin threads) (eager : bool)
+    : Exec.t mstate string () :=
+    (* Check if the thread is already marked terminated, in which case there
+      is no transition to take. *)
+    terminated ← mget ((.!!! tid) ∘ termThreads);
+    guard_discard (negb terminated);;
+
+    (* Run one instruction *)
+    cinterp (run_outcome tid eager) isem;;
+    (* Check if the thread is actually terminated and mark it if so *)
+    'regs ← mget ((.!!! tid) ∘ regs);
+    if term tid regs then
+      (* Mark it as terminated *)
+      msetv ((.!!! tid) ∘ termThreads) true
+    else
+      mret ().
+
+  (** ** Top level transitions *)
+
+  (** This returns [Some tid] when taking a instruction transition because it
+      might enable eager transitions *)
+  Definition step : Exec.t mstate string (option (fin threads)) :=
     (* The transition taken is either a flush to memory or a run_outcome call,
-     for a specific tid *)
+    for a specific tid *)
     tid ← mchoosef;
     flush_transition ← mchoosef;
     if (flush_transition : bool) then
       (* This function discards if there is nothing to flush. *)
-      flush_one_item_buffer tid
+      flush_one_item_buffer tid;;
+      mret None
     else
-      (* Check if the thread is already marked terminated, in which case there
-       is no transition to take. *)
-      terminated ← mget ((.!!! tid) ∘ termThreads);
-      guard_discard (negb terminated);;
+      execution_step tid false;;
+      mret (Some tid).
 
-      (* Run one instruction *)
-      cinterp (run_outcome tid) isem;;
-      (* Check if the thread is actually terminated and mark it if so *)
-      'regs ← mget ((.!!! tid) ∘ regs);
-      if term tid regs then
-        (* Mark it as terminated *)
-        msetv ((.!!! tid) ∘ termThreads) true
-      else mret ().
+  (** ** Eager transition functions *)
+  Definition run_eager_thread_step (tid : fin threads) :
+      Exec.t mstate string bool :=
+    (* Eagerly run single thread instruction if possible.
+      The returned bool is true if the instruction runs successfully *)
+    '(terminated : bool) ← mget ((.!!! tid) ∘ termThreads);
+    if terminated then
+      mret false
+    else
+      st ← mGet;
+      (* Run instruction eagerly. Only bind new outcome if it is successful *)
+      let new_outcome := execution_step tid true st in
+        if Exec.to_result_list new_outcome is [] then
+          mret false
+        else
+          Exec.lift_res_st new_outcome;;
+          mret true.
+
+  Fixpoint run_eager_thread (fuel : nat) (tid : fin threads) :
+      Exec.t mstate string nat :=
+    (* Run as many instructions as possible for this thread *)
+    if fuel is S fuel then
+      (* Run instruction eagerly if possible *)
+      '(instr_ran : bool) ← run_eager_thread_step tid;
+      if instr_ran then
+        run_eager_thread fuel tid
+      else mret (S fuel)
+    else mthrow "Out of fuel".
+
+  Definition run_eager_all (fuel : nat) : Exec.t mstate string nat :=
+    (* For each thread, run as many instructions as possible *)
+    foldlM run_eager_thread fuel (enum (fin threads)).
+
+
+
+  (** * Lift to executable archModel *)
+
+  Definition from_archState (astate : archState threads) : mstate :=
+    {|
+      regs := astate.(archState.regs);
+      mem := astate.(archState.memory);
+      buf := Vector.const [] threads;
+      lock := None;
+      memWritten := ∅;
+      termThreads := vimap term astate.(archState.regs);
+    |}.
+
+  Definition to_archState (mstate : mstate) : option (archState threads) :=
+    if all_buffers_empty mstate && bool_decide (lock mstate = None) then
+      Some {|
+          archState.regs := regs mstate;
+          archState.memory := mem mstate;
+          archState.address_space := ()
+        |}
+    else None.
+
+  Definition to_terminated_archState (mstate : mstate) :
+      option {s : archState threads & archState.is_terminated term s} :=
+    guard (∀ tid, mstate.(termThreads) !!! tid : bool);;
+    astate ← (to_archState mstate);
+    if decide (archState.is_terminated term astate) is left p then
+      Some (existT astate p)
+    else None.
+
+  (** ** No-eager-transitions runner *)
+
+  (** Just take non-eager transition until reaching termination *)
+  Fixpoint run_to_term_no_eager (fuel : nat) :
+    Exec.t mstate string {s : archState threads & archState.is_terminated term s} :=
+    (* run until out of fuel or conditions met *)
+    if fuel is S fuel then
+      (* Run a non-eager execution step *)
+      step;;
+      (* Check if termination condition met. If not, execute non-eager step *)
+      fstate ← mget to_terminated_archState;
+      if fstate is Some fs then mret fs else run_to_term_no_eager fuel
+    else mthrow "Out of fuel".
+
+
+  (** ** Eager-transition-enabled runner *)
+
+  (** [run_to_term_eager_normal fuel] Assumes that no eager transition is
+      possible and does a normal transition.
+
+      [run_to_term_eager_eager fuel tid] Does all possible transition in thread
+      [tid] then goes back to the "normal" runner. *)
+  Fixpoint run_to_term_eager_normal (fuel : nat) :
+      Exec.t mstate string _ :=
+    (* run until out of fuel or conditions met *)
+    if fuel is S fuel then
+      (* Run a non-eager execution step *)
+      eager_thread ← step;
+      if eager_thread is Some tid then
+        run_to_term_eager_eager fuel tid
+      else
+        (* Check if termination condition met. If not, execute non-eager step *)
+        fstate ← mget to_terminated_archState;
+        if fstate is Some fs then mret fs else run_to_term_eager_normal fuel
+    else mthrow "Out of fuel"
+
+  with run_to_term_eager_eager (fuel : nat) (tid : fin threads)  :
+      Exec.t mstate string {s : archState threads & archState.is_terminated term s} :=
+    if fuel is S fuel then
+      (* Try to do eager execution of thread [tid] if possible *)
+      '(instr_ran : bool) ← run_eager_thread_step tid;
+      if instr_ran then
+        (* If we run an eager transition, run another one *)
+        run_to_term_eager_eager fuel tid
+      else
+        (* Otherwise, check if termination condition met. If not, execute
+            non-eager step *)
+        fstate ← mget to_terminated_archState;
+        if fstate is Some fs then mret fs else run_to_term_eager_normal fuel
+    else mthrow "Out of fuel".
+
+
+  (** ** Full model runner *)
+
+  Definition run_to_term (allow_eager : bool) (fuel : nat) :
+        Exec.t mstate string
+        {s : archState threads & archState.is_terminated term s} :=
+    (* If eager transitions allowed, try to eagerly execute each thread,
+        as we are in the first iteration *)
+    if allow_eager then
+      run_eager_all fuel;;
+      fstate ← mget to_terminated_archState;
+      if fstate is Some fs then mret fs else run_to_term_eager_normal fuel
+    else
+      run_to_term_no_eager fuel.
 End Model.
+Arguments mstate : clear implicits.
 
-(** * Lift to executable archModel *)
-
-Definition from_archState {nth} (term : terminationCondition nth)
-  (astate : archState nth) : machine_state nth :=
-  {|
-    regs := astate.(archState.regs);
-    mem := astate.(archState.memory);
-    buf := Vector.const [] nth;
-    lock := None;
-    memWritten := ∅;
-    termThreads := vimap term astate.(archState.regs)
-  |}.
-
-Definition to_archState {nth} (mstate : machine_state nth) : option (archState nth) :=
-  if all_buffers_empty mstate && bool_decide (lock mstate = None) then
-    Some {|
-        archState.regs := regs mstate;
-        archState.memory := mem mstate;
-        archState.address_space := ()
-      |}
-  else None.
-
-Fixpoint run_to_term {nth} (fuel : nat) (isem : iMon ())
-  (term : terminationCondition nth) :
-  Exec.t (machine_state nth) string {s : archState nth & archState.is_terminated term s} :=
-  (* run until out of fuel or conditions met *)
-  if fuel is S fuel then
-    step isem term;;
-    mstate ← mGet;
-    astate ← mget to_archState;
-    if astate is Some astate then
-      if decide (archState.is_terminated term astate) is left p then
-        mret (existT astate p)
-      else run_to_term fuel isem term
-    else run_to_term fuel isem term
-  else mthrow "Out of fuel".
 
 (** Top-level one-threaded model function that takes fuel (guaranteed
     termination) and an instruction monad, and returns a computational set of
     all possible final states. *)
-Definition x86_operational_modelc (fuel : nat) (isem : iMon ()) : (archModel.c ∅) :=
+Definition x86_operational_modelc (fuel : nat) (isem : iMon ()) (allow_eager : bool)
+  : (archModel.c ∅) :=
   λ n term (initSt: archState n),
     from_archState term initSt
-    |> archModel.Res.from_exec (run_to_term fuel isem term).
+    |> archModel.Res.from_exec (run_to_term isem term allow_eager fuel).
